Reprove all existing interop wrappers with new stack TCB

vale/code/arch/x64/interop/Vale.AsLowStar.MemoryHelpers.fst
@@ -37,9 +37,9 @@ let reveal_imm_readable (#src #t:_) (x:ibuf_t src t) (s:ME.mem) = ()
 let readable_live (#src #t:_) (x:buf_t src t) (s:ME.mem) = ()
 let readable_imm_live (#src #t:_) (x:ibuf_t src t) (s:ME.mem) = ()
 let buffer_readable_reveal #max_arity #n src bt x args h0 stack = ()
-let get_heap_mk_mem_reveal #max_arity #n args h0 stack = ()
-let buffer_as_seq_reveal #max_arity #n src t x args h0 stack = ()
-let immbuffer_as_seq_reveal #max_arity #n src t x args h0 stack = ()
+let get_heap_mk_mem_reveal #n args h0 stack = ()
+let buffer_as_seq_reveal #n src t x args h0 stack = ()
+let immbuffer_as_seq_reveal #n src t x args h0 stack = ()
 let buffer_as_seq_reveal2 src t x va_s = ()
 let immbuffer_as_seq_reveal2 src t x va_s = ()
 let buffer_addr_reveal src t x args h0 = ()
@@ -59,9 +59,11 @@ let core_create_lemma_taint_hyp
     #max_arity
     #arg_reg
     #n
-    (args:IX64.arity_ok max_arity arg)
+    (args:IX64.arg_list)
     (h0:HS.mem)
-    (stack:IX64.stack_buffer n{mem_roots_p h0 (arg_of_sb stack::args)})
+    (stack:IX64.stack_buffer n{
+      B.length stack >= n/8 + (List.Tot.length args - max_arity) + 5 /\
+      mem_roots_p h0 (arg_of_sb stack::args)})    
   : Lemma
       (ensures (let va_s = LSig.create_initial_vale_state #max_arity #arg_reg args h0 stack in
                 LSig.taint_hyp args va_s /\
@@ -70,7 +72,9 @@ let core_create_lemma_taint_hyp
     let taint_map = va_s.VS.memTaint in
     let s_args = arg_of_sb stack::args in
     let mem = va_s.VS.mem in
-    assert (mem == mk_mem s_args h0);
+    let h1 = IX64.stack_of_args max_arity (List.Tot.length args) args stack h0 in  
+    IX64.live_arg_modifies h0 h1 args stack;
+    assert (mem == mk_mem s_args h1);
     let raw_taint = IX64.(mk_taint s_args IX64.init_taint) in
     assert (taint_map == create_memtaint mem (args_b8 s_args) raw_taint);
     ME.valid_memtaint mem (args_b8 s_args) raw_taint;
@@ -116,16 +120,60 @@ let same_down_up_buffer_length src b =
   DV.length_eq db;
   FStar.Math.Lemmas.cancel_mul_div (B.length b) (view_n src)
 
+val lemma_mult_lt_right: a:pos -> b:nat -> c:nat -> Lemma
+  (requires (b < c))
+  (ensures  (b * a < c * a))
+let lemma_mult_lt_right a b c = 
+  assert (c <> 0);
+  if b = 0 then (
+    assert (0 * a == 0);
+    FStar.Math.Lemmas.pos_times_pos_is_pos c a
+  ) else (
+    FStar.Math.Lemmas.lemma_mult_lt_left a b c
+  )
+
 let down_up_buffer_read_reveal src h s b i =
   let db = get_downview b in
-  let n = view_n src in
+  let n:pos = view_n src in
   let up_view = (LSig.view_of_base_typ src) in
   let ub = UV.mk_buffer db up_view in
   same_down_up_buffer_length src b;
+  UV.length_eq ub;
   UV.get_sel h ub i;
+  lemma_mult_lt_right n i (DV.length db / n);
+  FStar.Math.Lemmas.multiply_fractions (DV.length db) n;
+  FStar.Math.Lemmas.nat_times_nat_is_nat i n;
   assert (low_buffer_read src src h b i == 
     UV.View?.get up_view (Seq.slice (DV.as_seq h db) (i*n) (i*n + n)));
   DV.put_sel h db (i*n);
   let aux () : Lemma (n * ((i*n)/n) == i*n) =
     FStar.Math.Lemmas.cancel_mul_div i n
   in aux()
+
+let same_buffer_same_upviews #src #bt b h0 h1 =
+    let dv = get_downview b in 
+    let s0 = DV.as_seq h0 dv in
+    let s1 = DV.as_seq h1 dv in
+    let aux (i:nat{i < DV.length dv}) : Lemma (Seq.index s0 i == Seq.index s1 i) =
+      DV.as_seq_sel h0 dv i;
+      DV.as_seq_sel h1 dv i;
+      DV.get_sel h0 dv i;
+      DV.get_sel h1 dv i
+    in Classical.forall_intro aux;
+    Seq.lemma_eq_intro s0 s1;
+    DV.length_eq dv;
+    BufferViewHelpers.lemma_uv_equal (LSig.view_of_base_typ bt) dv h0 h1
+
+let same_immbuffer_same_upviews #src #bt b h0 h1 =
+    let dv = get_downview b in 
+    let s0 = DV.as_seq h0 dv in
+    let s1 = DV.as_seq h1 dv in
+    let aux (i:nat{i < DV.length dv}) : Lemma (Seq.index s0 i == Seq.index s1 i) =
+      DV.as_seq_sel h0 dv i;
+      DV.as_seq_sel h1 dv i;
+      DV.get_sel h0 dv i;
+      DV.get_sel h1 dv i
+    in Classical.forall_intro aux;
+    Seq.lemma_eq_intro s0 s1;
+    DV.length_eq dv;
+    BufferViewHelpers.lemma_uv_equal (LSig.view_of_base_typ bt) dv h0 h1
