vale/code/arch/x64/interop/Vale.AsLowStar.MemoryHelpers.fsti
@@ -80,9 +80,8 @@ val buffer_readable_reveal
       List.memP (mut_to_b8 src x) (ptrs_of_mem mem))
 
 val get_heap_mk_mem_reveal
-  (#max_arity:_)
   (#n:_)
-  (args:IX64.arity_ok max_arity arg)
+  (args:IX64.arg_list)
   (h0:HS.mem)
   (stack:IX64.stack_buffer n{mem_roots_p h0 (arg_of_sb stack::args)}) : Lemma
   (let mem = mk_mem (arg_of_sb stack::args) h0 in
@@ -90,11 +89,10 @@ val get_heap_mk_mem_reveal
    MES.get_heap (as_vale_mem mem) == I.down_mem mem)
 
 val buffer_as_seq_reveal
-  (#max_arity:_)
   (#n:_)
   (src t:ME.base_typ)
   (x:buf_t src t)
-  (args:IX64.arity_ok max_arity arg)
+  (args:IX64.arg_list)
   (h0:HS.mem)
   (stack:IX64.stack_buffer n{mem_roots_p h0 (arg_of_sb stack::args)}) : Lemma
   (let y = as_vale_buffer x in
@@ -106,11 +104,10 @@ val buffer_as_seq_reveal
     (UV.as_seq h0 (UV.mk_buffer db (LSig.view_of_base_typ t))))
 
 val immbuffer_as_seq_reveal
-  (#max_arity:_)
   (#n:_)
   (src t:ME.base_typ)
   (x:ibuf_t src t)
-  (args:IX64.arity_ok max_arity arg)
+  (args:IX64.arg_list)
   (h0:HS.mem)
   (stack:IX64.stack_buffer n{mem_roots_p h0 (arg_of_sb stack::args)}) : Lemma
   (let y = as_vale_immbuffer x in
@@ -202,9 +199,11 @@ val core_create_lemma_taint_hyp
     (#max_arity:_)
     (#arg_reg:IX64.arg_reg_relation max_arity)
     (#n:_)
-    (args:IX64.arity_ok max_arity arg)
+    (args:IX64.arg_list)
     (h0:HS.mem)
-    (stack:IX64.stack_buffer n{mem_roots_p h0 (arg_of_sb stack::args)})
+    (stack:IX64.stack_buffer n{
+      B.length stack >= n/8 + (List.Tot.length args - max_arity) + 5 /\
+      mem_roots_p h0 (arg_of_sb stack::args)})
   : Lemma
       (ensures (let va_s = LSig.create_initial_vale_state #max_arity #arg_reg args h0 stack in
                 LSig.taint_hyp args va_s /\
@@ -298,3 +297,19 @@ val down_up_buffer_read_reveal (src:base_typ) (h:HS.mem) (s:ME.mem) (b:(buf_t sr
   (ensures LSig.nat_to_uint src (ME.buffer_read (as_vale_buffer b) i s) == 
     Seq.index (B.as_seq h b) i)
   [SMTPat (ME.buffer_read (as_vale_buffer b) i s); SMTPat (Seq.index (B.as_seq h b) i)]
+
+val same_buffer_same_upviews (#src #bt:base_typ) (b:buf_t src bt) (h0 h1:HS.mem) : Lemma
+  (requires Seq.equal (B.as_seq h0 b) (B.as_seq h1 b))
+  (ensures (
+    let db = get_downview b in
+    DV.length_eq db;
+    let ub = UV.mk_buffer db (LSig.view_of_base_typ bt) in
+    Seq.equal (UV.as_seq h0 ub) (UV.as_seq h1 ub)))
+
+val same_immbuffer_same_upviews (#src #bt:base_typ) (b:ibuf_t src bt) (h0 h1:HS.mem) : Lemma
+  (requires Seq.equal (B.as_seq h0 b) (B.as_seq h1 b))
+  (ensures (
+    let db = get_downview b in
+    DV.length_eq db;
+    let ub = UV.mk_buffer db (LSig.view_of_base_typ bt) in
+    Seq.equal (UV.as_seq h0 ub) (UV.as_seq h1 ub)))
